project/report/project-report.md
@@ -5,7 +5,7 @@
 # Formal Definition
 ## Syntax
 We start by defining the formal syntax of our extension of untyped Lambda Calculus, which we call *Lambda+*.
-The syntax is inspired from the one on Leroy's slides and *HOFL* (Higher Order Functional Language) seen in the course Principles for Software Composition
+The syntax is inspired by the one on Leroy's slides and *HOFL* (Higher Order Functional Language) seen in the course Principles for Software Composition:
 $$
 \begin{align}
 t ::=\ &x\ |\ n\ |\ b\  \\
@@ -21,23 +21,14 @@ where:
 - $\text{aop} \in \{+, -,\times\}$
 - $\text{bop}\in \{\land, \lor, =, \neq, >, <\}$ 
 
-De Bruijn indices are used to represent variable bindings.
-Instead of using variable names, De Bruijn indices encode the information about the scope of a variable by representing it as a number indicating how many lambdas must be traversed to reach its binding occurrence.
-
-Consider the following example: 
-$$(\lambda f.\lambda x.\lambda y.f\ x\ y) \equiv λ(λ(λ.2 1 0))$$
-- $\lambda f$: $f$ is not bound by any enclosing lambda, so it's represented by index 0.
-- $λx$: $x$ is bound by the enclosing $\lambda f$ abstraction, so it's represented by index $0$.
-- $λy$: $y$ is bound by the enclosing $\lambda x$ abstraction, and $x$ is bound by the enclosing $\lambda f$ abstraction. So $y$ is represented by index $1$, and $x$ is represented by index $0$.
-
-Therefore the set $Var$ is a set of De Bruijn indices. 
-
-An environment $\sigma$ is used to store the bindings and it is defined as a sequence of values.
-The value associated with the De Bruijn index $j$ will be $\rho[j]$.
-The admissible values of Lambda+ are integers, booleans, and closures. 
+**Observations:**
+1) De Bruijn indices are used to represent variable bindings. Therefore the set $Var$ is a set of De Bruijn indices. 
+2) The admissible values of Lambda+ are integers and booleans (and closures, to represent partial functions)
+3) We will define an "environment" as a sequence of values to store the bindings index-value
 ## Type System
 The above syntax allows *pre-terms*, terms that do not have a valid semantic.
-Consider $t = \text{if}\ 3\ \text{then}\ 1\ \text{else}\ 2$. It is clear that $t$ has not a valid semantic as the guard of the `if` command has to be evaluated in a boolean. 
+Consider $t = \text{if}\ 3\ \text{then}\ 1\ \text{else}\ 2$. It is clear that $t$ has not a valid semantic: the guard of the `if`
+command has to be a boolean. 
 
 There is the need to introduce a **type system** to distinguish pre-terms from terms. 
 Let's define the types of our values as follows
@@ -48,55 +39,56 @@ Then we assume that the variables are typed and that we have a *typing context* 
 - $Var = \{Var_\tau\}_{\tau\in \mathcal{T}}$
 - $\Gamma$ is a list or set of variable-type pairs. Each pair associates a variable with its type
 
-The type system, a set of inference rules using structural induction of the Lambda+ syntax, assigns to a pre-term a type, if possible. 
+The type system, a set of inference rules using structural induction of the Lambda+ syntax, assigns to each pre-term a type, if possible. 
 We use the type system to make type judgments, such as 
 $$t : \tau \iff \text{t has type}\ \tau$$
 A pre-term $t$ is **well-formed** if $\exists \tau\in \mathcal{T}. t : \tau$.
-In other words: if we can assign a type to a pre-term $t$ than $t$ is well-formed.
+In other words: if we can assign a type to a pre-term $t$ then $t$ is well-formed.
 
 The type system is made of the following inference rules: 
 ![[Screenshot from 2024-03-06 10-53-04.png | center | 600]]
 
-The above type system will be "embedded" in the following sections.
+The above type system will be "*embedded*" in the code of the interpreter.
 ## Semantics
 ### Small-Step Semantics
 Now we define the small-step semantics of **well-formed** Lambda+ terms. To simplify the notation we represent with $\mathbb{T}$ the set of all the possible well-formed terms. 
 We consider a structural operational semantics, i.e. specifying the execution recursively on syntax, in a machine-independent way. 
 
-To help us determine the semantic of a term we define a **store** function $\sigma:Var\rightarrow \mathbb{N}\ \cup\ \mathbb{B}$, and with $\mathbb{M}$ we represent the set of all possible stores $\sigma$.
+To help us determine the semantics of a term we define a **store** function $\sigma:Var\rightarrow \mathbb{N}\ \cup\ \mathbb{B}$, and with $\mathbb{M}$ we represent the set of all possible stores $\sigma$.
 We also define a function $\text{bind}$, that adds (on top) to the current environment (store) a new value. 
-Lambda calculus has no side effects, this is purely to make things easier in the actual implementation of the language.
 
-A program written in Lambda+ that terminates returns a value $v \in V= \{int, bool, closure(t, \rho)\}$.
-Since we will define a **bounded interpreter** with a fuel parameter that is decreased with each step we also have to consider the case that the fuel reaches $0$ before the program has terminated. 
+A program written in Lambda+ that terminates returns a value $v \in V= \{\text{int}, \text{bool}, \text{closure}(t, \rho)\}$.
+We will define a **bounded interpreter** with a fuel parameter that is decreased at each step, so every program technically terminates.
+Nonetheless, we have to consider the case where the fuel reaches $0$ before the program has terminated. 
 We then define the set of the possible values returned by a Lambda+ program as
 $$\bar{V} = V\ \cup \perp$$
-where $\perp$ is called **bottom**, the value of non-terminating programs (as diverging programs that never terminates). 
-Abusing the notation, we also use $\perp$ as a value of undefined variables. 
+where $\perp$ is called **bottom**, the value of non-terminating programs (as diverging programs that never terminate). 
+Abusing the notation, we also use $\perp$ to represent undefined variables and type errors. 
 
 We represent intermediate states of the computation as pairs $\langle t, \sigma\rangle \in \mathbb{T}\times\mathbb{M}$.
 Then we define a transition system $(S, \rightarrow)$  where the first is a set of states and the second is a transition system, where the transitions are of the form 
 $$\langle t, \sigma\rangle \rightarrow \langle t',\sigma'\rangle$$
 
-Mind that we distinguish between the syntactic operations and their actual semantic operations using an over line: 
+**Notation:** We distinguish between the syntactic operations and their actual semantic operations using an overline: 
 - $\text{aop}$ is syntax
 - $\overline{\text{aop}}$ is semantic
 
 **The small-step semantics of Lambda+ is defined by the following inference rules:** 
 ![[Pasted image 20240306155136.png | center | 560]]
+
 **Note:** For brevity not all the rules have been listed: 
-- The rules above are under the assumption that the program terminates and that every variable is always defined in $\sigma$. In reality there will be rules to cover the scenario in which a part of the program diverge or a lookup error, giving as result $\perp$ 
-- The rules for boolean expressions are basically identical to the one for arithmetic expression, hence are not shown
+- The rules above are under the assumption that the program terminates and that every variable is always defined in $\sigma$. In reality, there will be rules to cover the scenario in which a part of the program diverges or a lookup error, giving as result $\perp$ 
+- The rules for boolean expressions are identical to the ones for arithmetic expressions, hence are not shown
 ### Big-Step Semantics
 To define the big-step semantics we build upon the small-step semantics. 
-A big-step computation is denoted with $\longrightarrow$ instead that the $\rightarrow$ used for the small-step.
+A big-step computation is denoted with $\longrightarrow$ instead of the $\rightarrow$ used for the small-step.
 
 **The big-step semantics of Lambda+ is defined by the following inference rules:** 
 ![[Pasted image 20240307094654.png | center | 560]]
 **Note:** For brevity not all the rules have been listed: 
-- Some rules (e.g., the rule for the lambda abstraction) remain the same and not showed
-- The rules above are under the assumption that the program terminates, i.e., we have enough fuel. In reality there will be rules to cover the scenario in which a part of the program diverge, giving as result $\perp$ 
-- The rules for boolean expressions are basically identical to the one for arithmetic expression, hence are not shown
+- Some rules (e.g., the rule for the lambda abstraction) remain the same and not listed
+- The rules above are under the assumption that the program terminates, i.e., we have enough fuel. In reality there will be rules to cover the scenario in which a part of the program diverges, giving as a result $\perp$ 
+- The rules for boolean expressions are identical to the ones for arithmetic expressions, hence are not shown
 ### Properties of the Semantics
 #### Determinism
 Is it true that two different "computations", on the same term and environment, always produce the same value?
@@ -107,19 +99,19 @@ And we ask ourselves if is it true that $\forall t . P(t)$.
 
 Assuming that the term is not diverging (e.g., it can be computed in a finite fuel) we could provide a formal proof using the Rule Induction Principle.
 #### Termination
-Is it true that every term terminates? This is immediately not true as we can define a term that always diverge, no matter the amount of fuel we provide. 
+Is it true that every term terminates? This is immediately not true as we can define a term that always diverges, no matter the amount of fuel we provide. 
 The lambda expression
 $$(\lambda x.x\ x)(\lambda x. x\ x)$$
-is the infinitely self applying function that never terminates, and it can be defined in Lambda+. 
+is the infinitely self-applying function that never terminates, and it can be defined in Lambda+. 
 # Definitional Interpreter 
-We can represent the provided definitional interpreter as a function, in a way that resemble what we would do for defining denotational semantics. 
+We can represent the provided definitional interpreter as a function, in a way that resembles what we would do for defining denotational semantics. 
 
 We introduce the function $[[\cdot]]_I: (\mathbb{Z}, \mathbb{M}, \mathbb{T}) \rightarrow (V \cup \{\perp\})$ as the *interpreter function*, where: 
 - the first argument is the remaining fuel
 - the second argument is the current store
 - the third argument is the term currently being interpreted
 
-The interpreter function the mathematical representation of the `eval` function defined in the attached source code, and it is defined as follows: 
+The interpreter function is the mathematical representation of the `eval` function defined in the attached source code, and it is defined as follows: 
 $$
 \begin{align}
 & [[(0,\ \_,\ \_)]]_I\ =\ \perp \\
@@ -151,9 +143,9 @@ $$
 Now we want to prove that the interpreter is **sound:**
 $$\forall n, t, v, \sigma. ([[(n, \sigma, t)]] = v \implies \langle t, \sigma\rangle\longrightarrow v)$$
 We prove that statement by induction on $t$. 
-**The base cases, where $t$ is either a variable, an integer or a boolean, are immediate to see.** 
+**The base cases, where $t$ is either a variable, an integer, or a boolean, are immediate to see.** 
 
-Let's now consider (two of the) more complex cases. 
+Let's now consider some complex cases. 
 **If Than Else:**
 $$\text{if}\ t\ \text{then}\ t_0\ \text{else}\ t_1$$
 **Note:** we consider only the case where $t$ evaluates to $true$, as the other case is analogous.
@@ -185,7 +177,7 @@ Using the hypothesis of the application:
 We proceed by the definition of $[[\cdot]]$ and we get that: $$[[(n, \sigma, t_0\ t_1)]] = [[(n, \sigma', t_0)]]$$
 And we want to prove that:
 $$\forall n, t, \overline{v}, \sigma'. ([[(n, \sigma', t)]] = \overline{v} \implies \langle t, \sigma'\rangle\longrightarrow \overline{v})$$
-Which is true by considering the three inductive hypothesis 1), 2) and 3) that makes applicable the hypothesis of the inference rule of the application.
+Which is true by considering the three inductive hypotheses 1), 2), and 3) that make applicable the hypothesis of the inference rule of the application.
 ## Completeness
 Completeness is defined as follows: 
 $$\forall t, \sigma, v. \exists n. \langle t, \sigma\rangle \longrightarrow v \implies [[(n, \sigma, t)]] =v$$
@@ -198,8 +190,8 @@ To compile and execute our code in the virtual machine we need to:
 	- define an interpreter for that language
 2) define a compilation step for our code that transforms a program written in Lambda+ in the code that the VM executes, similar to the transformation of Java to Bytecode
 
-Continuing the similarities with Java, our virtual machine will be a stack-based machine, its computation will be performed on an operand stack, in a way that resembles the JVM. 
-To keep things manageable the stack is used as an operand stack and as a call stack, but in our case the "activation records" only stores the return address and the environment. 
+Continuing the similarities with Java, our virtual machine will be stack-based, its computation will be performed on an operand stack, in a way that resembles the JVM. 
+To keep things manageable the stack is used as an operand stack and as a call stack, but in our case, the "activation records" only store the return address and the environment. 
 ## Virtual Machine
 We start by defining the syntax for the language of our virtual machine:
 $$
@@ -219,7 +211,7 @@ We provide a small-step semantic where the intermediate step is the triple $\lan
 - $\gamma$ is the operand/call stack
 
 **Notation:** 
-1) A program is seen as a sequence of commands. We decide that the last command before the termination will always be a $\text{Skip}$. This is to make easier to identify the end of a program: a program has reached its end when it is no more a sequence of commands, and the remaining command is a $\text{Skip}$. We will present an inference rule for enforcing every non-skip command into a sequence where the last command $\text{Skip}$  
+1) A program is seen as a sequence of commands. We decide that the last command before the termination will always be a $\text{Skip}$. This is to make it easier to identify the end of a program: a program has reached its end when it is no more a sequence of commands, and the remaining command is a $\text{Skip}$. We will present an inference rule for enforcing every non-skip command into a sequence where the last command $\text{Skip}$  
 2) We represent the final state of the VM as a single value. 
 3) We use $v :: \sigma$ to represent the insertion/presence of $v$ on top of the stack. 
 4) We use the bottom symbol $\perp$ for representing errors. 
@@ -228,13 +220,13 @@ We provide a small-step semantic where the intermediate step is the triple $\lan
 ![[IMG_0441.png | center | 700]]
 
 **Note:** For brevity not all the rules have been listed: 
-- The rules for $\text{BOP}$ are basically identical to the one for arithmetic operations, hence are not shown
-- As we did for Lambda+ we here presents only the rules for "correct" programs (rules that do not give $\perp$)
+- The rules for $\text{BOP}$ are basically identical to the ones for arithmetic operations, hence are not shown
+- As we did for Lambda+ we here present only the rules for "correct" programs (rules that do not give $\perp$)
 - The $\langle \text{Skip};C, \sigma,\gamma\rangle$ is not listed as the semantics of a "non-final" is trivial
 ## Compilation of Lambda+
 We now present the compilation step that transforms a program written in *Lambda+* to the language of the virtual machine.
 
-We proceed in a similar way of the "interpretation function" and define the "compilation function" as a function that goes from well-formed Lambda+ terms to $C$: $$[[\cdot]]_C : \mathbb{T}\rightarrow (C \cup \{\perp\})$$
+We proceed in a similar way to the "interpretation function" and define the "compilation function" as a function that goes from well-formed Lambda+ terms to $C$: $$[[\cdot]]_C : \mathbb{T}\rightarrow (C \cup \{\perp\})$$
 The function $[[\cdot]]_C$ is defined by cases as follows: 
 $$
 \begin{align}
@@ -267,4 +259,4 @@ $$
 \end{align}
 $$
 # Project Delivery
-The file `lambda_plus.v` implements all content in the following report.
+The file `lambda_plus.v` implements all the content described in this report. 
